limit implementation

theories/Compositional_Structures/Basic_Modules/Component_Types/Social_Choice_Types/Ballot_Refinement.thy
@@ -65,27 +65,43 @@ lemma is_less_preferred_than_ref:
   apply (refine_vcg)
   by (auto simp only: refine_rel_defs less_preffered_l_rel_eq)
 
+find_theorems filter
 
 lemma limitref:
   shows "(limit_l, limit) \<in> \<langle>Id\<rangle>alt_set_rel \<rightarrow> ballot_rel \<rightarrow> ballot_rel"
   apply (refine_vcg, rename_tac A' A bl br)
-  apply (auto simp add: refine_rel_defs)
-sorry
-(*proof -
-  fix A' A :: "'a set"
+proof -
+    fix A' A :: "'a set"
   fix bl :: "'a Preference_List"
   fix  br :: "'a Preference_Relation"
-  assume brel: "(bl, br) \<in> ballot_rel"
   assume arel: "(A', A) \<in> \<langle>Id\<rangle>alt_set_rel"
-  from arel have aeq: "A' = A" by (auto simp add: alt_set_rel_def in_br_conv)
-  from arel have fina: "finite A'" by (auto simp add: alt_set_rel_def in_br_conv)
-  from brel have wf: "well_formed_pl bl" by (simp add: in_br_conv)
-  have "limit A br = pl_\<alpha> (limit_l A bl)"
-    using brel  apply (induction bl)
-     apply (auto simp add: brel wf)
-
-  (* inductctive proof with case distinction  *) 
+  assume bid: "(bl, br) \<in> ballot_rel"
+  from this have eq: "br = pl_\<alpha> bl" by (simp add: in_br_conv)
+  from bid have prec: "distinct bl" using well_formed_pl_def in_br_conv
+      by (metis)
+  from prec have "(limit_l A bl, limit A (pl_\<alpha> bl)) \<in> ballot_rel"
+  proof (induct bl)
+   show "(limit_l A [], limit A (pl_\<alpha> [])) \<in> ballot_rel"
+    apply (auto simp add: pl_\<alpha>_def List.member_def)
+    unfolding pl_\<alpha>_def well_formed_pl_def
+    using in_br_conv
+    by (metis (no_types, lifting) Collect_empty_eq case_prodE distinct.simps(1) is_less_preferred_than_l.elims(2) member_rec(2))
+next
+  fix a :: "'a"
+  fix bbl:: "'a Preference_List"
+  assume ic: "(distinct bbl \<Longrightarrow> (limit_l A bbl, limit A (pl_\<alpha> bbl)) \<in> ballot_rel)"
+  assume precc: "distinct (a # bbl)"
+  from this have dc: "distinct (bbl)" by auto
+  have infil: "a \<notin> A \<longrightarrow> filter (\<lambda>a. a \<in> A) (a#bbl) = filter (\<lambda>a. a \<in> A) (bbl) "
+    by auto
+  from infil dc ic have "a \<notin> A \<longrightarrow> (limit_l A (a # bbl), limit A (pl_\<alpha> (bbl))) \<in> ballot_rel"
+    unfolding limit_l.simps  well_formed_pl_def
+    by presburger
+  oops
+  
+  (* inductctive proof with case distinction 
 qed*)
+
 
 definition "limit_monadic_inv A ballot \<equiv> \<lambda> (b, newb).
   b = drop (length ballot - length b) ballot
@@ -93,91 +109,51 @@ definition "limit_monadic_inv A ballot \<equiv> \<lambda> (b, newb).
 
 definition  limit_monadic :: "'a set \<Rightarrow> 'a Preference_List \<Rightarrow> 'a Preference_List nres" where
 "limit_monadic A ballot \<equiv> do {
-  (_,newb) <-  WHILEIT (limit_monadic_inv A ballot) (FOREACH_cond (\<lambda>_.True)) 
-    (FOREACH_body  (\<lambda> x newb. 
-    RETURN  (if x \<in> A then (op_list_append newb x) else (newb)) 
-  )) (ballot,[]); 
-  RETURN newb}"
+    ((i, nbal), bal) \<leftarrow> WHILET
+  (\<lambda>((i, nbal), bal). i < length bal) 
+      (\<lambda>((i, nbal), bal). do {
+      ASSERT (i < (length bal));
+      c <- mop_list_get (bal) i;
+      if (c \<in> A) then
+        RETURN ((i + 1,op_list_append nbal c), bal)
+      else
+        RETURN ((i + 1, op_list_copy nbal), bal)
+    })((0, []), ballot);
+    RETURN (nbal)
+  }"                          
 
-definition  limit_nfoldli:: "'a set \<Rightarrow> 'a Preference_List \<Rightarrow> 'a Preference_List nres" where
-"limit_nfoldli A ballot \<equiv> 
-  nfoldli ballot (\<lambda>_.True) 
-    (\<lambda> x newb. 
-    RETURN  (if x \<in> A then ( newb @ [x]) else (newb)) 
-  ) []"
+
 
 lemma limitnref:
-  shows "(limit_nfoldli, (\<lambda> A br. SPEC(\<lambda> lim. pl_\<alpha> lim = (limit A br)))) \<in> \<langle>Id\<rangle>alt_set_rel \<rightarrow>
-     ballot_rel \<rightarrow> \<langle>Id\<rangle>nres_rel"
-  unfolding limit_nfoldli_def
-  apply (refine_rcg, rename_tac A' A bl br)
-proof -
-  fix A' A :: "'a set"
-  fix bl :: "'a Preference_List"
-  fix  br :: "'a Preference_Relation"
-  assume brel: "(bl, br) \<in> ballot_rel"
-  assume arel: "(A', A) \<in> \<langle>Id\<rangle>alt_set_rel"
-  from arel have aeq: "A' = A" by (auto simp add: alt_set_rel_def in_br_conv)
-  from arel have fina: "finite A'" by (auto simp add: alt_set_rel_def in_br_conv)
-  from brel have dis: "distinct bl" using in_br_conv
-    by (metis well_formed_pl_def)
-  show  "nfoldli bl (\<lambda>_. True) (\<lambda>x newb. RETURN (if x \<in> A' then newb @ [x] else newb)) []
-       \<le> SPEC (\<lambda>lim. pl_\<alpha> lim = limit A br)"
-  proof (simp add: aeq, refine_vcg nfoldli_rule[where I = 
-        "(\<lambda> proc xs newb. (pl_\<alpha> newb) = (limit A (pl_\<alpha> proc))
-          \<and> set newb \<subseteq> set proc)"])
-    show "pl_\<alpha> [] = limit A (pl_\<alpha> [])"
-    unfolding pl_\<alpha>_def
-    by (simp add: List.member_def)
-  next
-    fix x :: 'a
-    fix l1 l2 :: "'a Preference_List"
-    fix si :: "'a Preference_List"
-    assume blsep: "bl = l1 @ x # l2"
-    assume " pl_\<alpha> si = limit A (pl_\<alpha> l1) \<and> set si \<subseteq> set l1"
-    from this have sub: "set si \<subseteq> set l1" by simp
-    from sub show "pl_\<alpha> (if x \<in> A then si @ [x] else si) = limit A (pl_\<alpha> (l1 @ [x]))"
-      using pl_\<alpha>_def 
-      apply auto
-      sorry
-  next
-    fix si
-    assume " \<not> True" 
-    thus "pl_\<alpha> si = limit A br" by simp
-  next
-    fix si
-    assume newp: "pl_\<alpha> si = limit A (pl_\<alpha> bl)"
-    from brel have "br = (pl_\<alpha> bl)"
-      by (simp add: in_br_conv)
-    from newp this show "pl_\<alpha> si = limit A br"
-      by simp
-  qed
-qed
- 
-lemma limitref:
-  shows "(limit_monadic, (\<lambda> A br. SPEC(\<lambda> lim. pl_\<alpha> lim = (limit A br)))) \<in> \<langle>Id\<rangle>alt_set_rel \<rightarrow>
-     ballot_rel \<rightarrow> \<langle>Id\<rangle>nres_rel"
+  shows "(limit_monadic, (\<lambda> A bl. SPEC(\<lambda> lim. lim = (limit_l A bl)))) \<in> \<langle>Id\<rangle>alt_set_rel \<rightarrow>
+      \<langle>Id\<rangle>list_rel \<rightarrow> \<langle>Id\<rangle>nres_rel"
   unfolding limit_monadic_def
   apply (refine_rcg, rename_tac A' A bl br)
 proof -
   fix A' A :: "'a set"
   fix bl :: "'a Preference_List"
-  fix  br :: "'a Preference_Relation"
-  assume brel: "(bl, br) \<in> ballot_rel"
+  fix  br :: "'a Preference_List"
   assume arel: "(A', A) \<in> \<langle>Id\<rangle>alt_set_rel"
-  have "  WHILE\<^sub>T\<^bsup>limit_monadic_inv A' bl\<^esup> (FOREACH_cond (\<lambda>_. True))
-        (FOREACH_body (\<lambda>x newb. RETURN (if x \<in> A' then op_list_append newb x else newb))) (bl, []) \<bind>
-       (\<lambda>(_, newb). RETURN newb)
-       \<le> SPEC (\<lambda>lim. pl_\<alpha> lim = limit A br) "
-    apply (refine_vcg WHILET_rule)
+  assume bid: "(bl, br) \<in> \<langle>Id\<rangle>list_rel"
+  from arel have aeq: "A' = A" by (auto simp add: alt_set_rel_def in_br_conv)
+  from arel have fina: "finite A'" by (auto simp add: alt_set_rel_def in_br_conv)
+  from bid have beq: "bl = br"
+    by simp 
+  show  " nfoldli bl (\<lambda>_. True) (\<lambda>x newb. RETURN (if x \<in> A' then (op_list_append newb x) else newb)) []
+       \<le> SPEC (\<lambda>lim. lim = limit_l A br)"
+    apply (refine_vcg nfoldli_rule[where I =
+        "(\<lambda> proc xs newb. newb = filter (\<lambda>x. x\<in> A) proc)"])
+    unfolding pl_\<alpha>_def
+    by (auto simp add: beq aeq)
+  oops
   
 
 sepref_definition limit_imp is "uncurry (limit_monadic)" ::
-  "(hs.assn nat_assn)\<^sup>k *\<^sub>a (list_assn nat_assn)\<^sup>k \<rightarrow>\<^sub>a  (arl_assn nat_assn)"
+  "(hs.assn nat_assn)\<^sup>k *\<^sub>a (arl_assn nat_assn)\<^sup>k \<rightarrow>\<^sub>a (arl_assn nat_assn)"
   unfolding limit_monadic_def
-  apply (rewrite in "\<hole>" arl.fold_custom_empty)
-  apply sepref_dbg_keep
-  done
+  apply (rewrite in "WHILET  _ _ (_, \<hole>)" op_list_copy_def[symmetric])
+  apply (rewrite in "WHILET _ _ \<hole>" arl.fold_custom_empty)
+  by sepref
 
 abbreviation "profile_rel \<equiv> \<langle>ballot_rel\<rangle>list_rel"
 abbreviation "profile_on_A_rel A \<equiv> \<langle>ballot_on_A_rel A\<rangle>list_rel"
